Fixed some pearlite

examples/pearlite-example/src/pearlite_example.rs
@@ -1,14 +1,22 @@
-#[cfg(not(feature = "hacspec"))]
-extern crate hacspec_lib;
+// #[cfg(not(feature="hacspec"))]
+// extern crate creusot_contracts;
+// #[cfg(not(feature="hacspec"))]
+// use creusot_contracts::*;
+
+// #[cfg(not(feature = "hacspec"))]
+// extern crate hacspec_attributes;
+// #[cfg(feature = "hacspec")]
+// use hacspec_attributes::*;
 
 use hacspec_lib::*;
 
-// #[cfg(not(feature = "hacspec"))]
-// use creusot_contracts::{ensures, requires};
-
-#[requires(x == y)]
-#[ensures(!(result == false))]
-pub fn ensure_something (x : u8, y : u8) -> bool {
-    x == y
+// Prove that this function implements the sum of the first n natural numbers.
+// Hint: there exists a closed form of this sum
+#[ensures(result == n * (n - 1_usize) / 2_usize)]
+pub fn sum_first_n(n: usize) -> usize {
+    let mut sum = 0;
+    for i in 0..n {
+        sum = sum + i;
+    }
+    sum
 }
-
