coq/src/Pearlite_Example.v
@@ -9,12 +9,20 @@ Open Scope hacspec_scope.
 Require Import Hacspec_Lib.
 Export Hacspec_Lib.
 
-Definition ensure_something (x_0 : int8) (y_1 : int8)  `{x_0 = y_1} : bool :=
-  (x_0) =.? (y_1).
+Definition sum_first_n (n_0 : uint_size)  : uint_size :=
+  let sum_1 : uint_size :=
+    usize 0 in 
+  let sum_1 :=
+    foldi (usize 0) (n_0) (fun i_2 sum_1 =>
+      let sum_1 :=
+        (sum_1) + (i_2) in 
+      (sum_1))
+    sum_1 in 
+  sum_1.
 
-Theorem ensures_ensure_something : forall result_2 (x_0 : int8) (y_1 : int8),
- forall {H_0 : x_0 = y_1},
- @ensure_something x_0 y_1 H_0 = result_2 ->
- ~ (result_2 = false).
+
+Theorem ensures_sum_first_n : forall result_3 (n_0 : uint_size),
+ @sum_first_n n_0 = result_3 ->
+ result_3 = ((n_0) * ((n_0) - (usize 1))) / (usize 2).
  Proof. Admitted.
 
